tests/lean/inductionErrors.lean
@@ -10,13 +10,13 @@ theorem ex1 (p q : Nat) : p ≤ q ∨ p > q := by
   cases p, q using elimEx with
   | lower d => apply Or.inl -- Error
   | upper d => apply Or.inr -- Error
-  | diag    => apply Or.inl; apply Nat.leRefl
+  | diag    => apply Or.inl; apply Nat.le_refl
 
 theorem ex2 (p q : Nat) : p ≤ q ∨ p > q := by
   cases p, q using elimEx2 with -- Error
   | lower d => apply Or.inl
   | upper d => apply Or.inr
-  | diag    => apply Or.inl; apply Nat.leRefl
+  | diag    => apply Or.inl; apply Nat.le_refl
 
 theorem ex3 (p q : Nat) : p ≤ q ∨ p > q := by
   cases p /- Error -/ using elimEx with
@@ -28,7 +28,7 @@ theorem ex4 (p q : Nat) : p ≤ q ∨ p > q := by
   cases p using Nat.add with -- Error
   | lower d => apply Or.inl
   | upper d => apply Or.inr
-  | diag    => apply Or.inl; apply Nat.leRefl
+  | diag    => apply Or.inl; apply Nat.le_refl
 
 theorem ex5 (x : Nat) : 0 + x = x := by
   match x with
@@ -58,19 +58,19 @@ theorem ex8 (p q : Nat) : p ≤ q ∨ p > q := by
   cases p, q using elimEx with
   | lower d => apply Or.inl; admit
   | upper2 /- Error -/ d => apply Or.inr
-  | diag    => apply Or.inl; apply Nat.leRefl
+  | diag    => apply Or.inl; apply Nat.le_refl
 
 theorem ex9 (p q : Nat) : p ≤ q ∨ p > q := by
   cases p, q using elimEx with
   | lower d => apply Or.inl; admit
   | _ => apply Or.inr; admit
-  | diag    => apply Or.inl; apply Nat.leRefl
+  | diag    => apply Or.inl; apply Nat.le_refl
 
 theorem ex10 (p q : Nat) : p ≤ q ∨ p > q := by
   cases p, q using elimEx with
   | lower d => apply Or.inl; admit
   | upper d => apply Or.inr; admit
-  | diag    => apply Or.inl; apply Nat.leRefl
+  | diag    => apply Or.inl; apply Nat.le_refl
   | _  /- error unused -/ => admit
 
 theorem ex11 (p q : Nat) : p ≤ q ∨ p > q := by
@@ -78,4 +78,4 @@ theorem ex11 (p q : Nat) : p ≤ q ∨ p > q := by
   | lower d => apply Or.inl; admit
   | upper d => apply Or.inr; admit
   | lower d /- error unused -/ => apply Or.inl; admit
-  | diag    => apply Or.inl; apply Nat.leRefl
+  | diag    => apply Or.inl; apply Nat.le_refl
