tests/lean/interactive/plainTermGoal.lean
@@ -1,11 +1,11 @@
-
+--
 example : 0 < 2 :=
-  Nat.ltTrans Nat.zeroLtOne (Nat.ltSuccSelf _)
-           --^ $/lean/plainTermGoal
+  Nat.lt_trans Nat.zero_lt_one (Nat.lt_succ_self _)
             --^ $/lean/plainTermGoal
              --^ $/lean/plainTermGoal
-                           --^ $/lean/plainTermGoal
-                                          --^ $/lean/plainTermGoal
+              --^ $/lean/plainTermGoal
+                             --^ $/lean/plainTermGoal
+                                              --^ $/lean/plainTermGoal
 
 example : OptionM Unit := do
   let y : Int ← none
@@ -14,14 +14,14 @@ example : OptionM Unit := do
   return ()
 
 example (m n : Nat) : m < n :=
-  Nat.ltTrans _ _
-              --^ $/lean/plainTermGoal
+  Nat.lt_trans _ _
+               --^ $/lean/plainTermGoal
 
 example : True := sorry
                 --^ $/lean/plainTermGoal
 
 example : ∀ n, n < n + 42 :=
-  fun n => Nat.ltOfLeOfLt (Nat.leAddRight n 41) (Nat.ltSuccSelf _)
+  fun n => Nat.lt_of_le_of_lt (Nat.le_add_right n 41) (Nat.lt_succ_self _)
 --^ $/lean/plainTermGoal
     --^ $/lean/plainTermGoal
 
@@ -29,7 +29,7 @@ example : ∀ n, n < 1 + n := by
   intro n
   rw [Nat.add_comm]
     --^ $/lean/plainTermGoal
-  exact Nat.ltSuccSelf _
+  exact Nat.lt_succ_self _
       --^ $/lean/plainTermGoal
 
 #check fun (n m : Nat) => m
