tests/lean/modBug.lean
@@ -1,1 +1,1 @@
-theorem proofOfFalse : False := Nat.zeroNeOne (Nat.mod_zero 1)
+theorem proofOfFalse : False := Nat.zero_ne_one (Nat.mod_zero 1)
