tests/lean/run/394.lean
@@ -1,7 +1,7 @@
 def casesTFOn {motive : Prop → Sort _} (P) [inst : Decidable P] : (T : motive True) → (F : motive False) → motive P :=
   λ ht hf => match inst with
-  | isTrue H => eqTrue H ▸ ht
-  | isFalse H => eqFalse H ▸ hf
+  | isTrue H => eq_true H ▸ ht
+  | isFalse H => eq_false H ▸ hf
 
 example (P) [Decidable P] : ¬¬P → P := by
   induction P using casesTFOn
