tests/lean/run/matrix.lean
@@ -33,14 +33,14 @@ macro_rules
   | `($x[$i, $j]) => `($x $i $j)
 
 def dotProduct [Mul α] [Add α] [Zero α] (u v : Fin m → α) : α :=
-  loop m (Nat.leRefl ..) Zero.zero
+  loop m (Nat.le_refl ..) Zero.zero
 where
   loop (i : Nat) (h : i ≤ m) (acc : α) : α :=
     match i, h with
     | 0, h   => acc
     | i+1, h =>
-      have : i < m := Nat.ltOfLtOfLe (Nat.ltSuccSelf _) h
-      loop i (Nat.leOfLt this) (acc + u ⟨i, this⟩ * v ⟨i, this⟩)
+      have : i < m := Nat.lt_of_lt_of_le (Nat.lt_succ_self _) h
+      loop i (Nat.le_of_lt this) (acc + u ⟨i, this⟩ * v ⟨i, this⟩)
 
 instance [Zero α] : Zero (Matrix m n α) where
   zero _ _ := 0
