tests/lean/simpArgTypeMismatch.lean
@@ -1,3 +1,3 @@
 example (p : Prop) [Decidable p] (hnp : ¬ p) :
     if decide p then 0 = 1 else 1 = 1 := by
-  simp [hnp, decideEqFalse Unit]
+  simp [hnp, decide_eq_false Unit]
